common.v
@@ -1,0 +1,25 @@
+From WR Require Import syntax typing.
+From Coq Require Import ssreflect.
+Require Import Psatz.
+
+Definition good_renaming ξ n Γ m Δ :=
+  (forall i, i < n -> ξ i < m /\ ren_tm ξ (dep_ith Γ i) = dep_ith Δ (ξ i)).
+
+Lemma good_renaming_truncate n m Γ :
+  good_renaming (Nat.add n) m (Nat.add n >> Γ) (n + m) Γ .
+Proof.
+  rewrite /good_renaming.
+  split.
+  - lia.
+  - asimpldep.
+    f_equal. fext => *; asimpl; lia.
+Qed.
+
+Lemma good_renaming_truncate' n m Γ :
+  n <= m ->
+  good_renaming (Nat.add n) (m - n) (Nat.add n >> Γ) m Γ.
+Proof.
+  move => h.
+  replace m with (n + (m - n)) at 2; last by lia.
+  apply good_renaming_truncate.
+Qed.
